cfrontend/SimplExpr.v
@@ -139,43 +139,6 @@ Definition transl_incrdecr (id: incr_or_decr) (a: expr) (ty: type) : expr :=
   | Decr => Ebinop Osub a (Econst_int Int.one type_int32s) (incrdecr_type ty)
   end.
 
-(** Generate a [Sset] or [Sbuiltin] operation as appropriate
-  to dereference a l-value [l] and store its result in temporary variable [id]. *)
-
-Definition chunk_for_volatile_type (ty: type) : option memory_chunk :=
-  if type_is_volatile ty
-  then match access_mode ty with By_value chunk => Some chunk | _ => None end
-  else None.
-
-Definition make_set (id: ident) (l: expr) : statement :=
-  match chunk_for_volatile_type (typeof l) with
-  | None => Sset id l
-  | Some chunk =>
-      let typtr := Tpointer (typeof l) noattr in
-      Sbuiltin (Some id) (EF_vload chunk) (Tcons typtr Tnil) ((Eaddrof l typtr):: nil)
-  end.
-
-(** Translation of a "valof" operation.
-  If the l-value accessed is of volatile type, we go through a temporary. *)
-
-Definition transl_valof (ty: type) (l: expr) : mon (list statement * expr) :=
-  if type_is_volatile ty
-  then do t <- gensym ty; ret (make_set t l :: nil, Etempvar t ty)
-  else ret (nil, l).
-
-(** Translation of an assignment. *)
-
-Definition make_assign (l r: expr) : statement :=
-  match chunk_for_volatile_type (typeof l) with
-  | None =>
-      Sassign l r
-  | Some chunk =>
-      let ty := typeof l in
-      let typtr := Tpointer ty noattr in
-      Sbuiltin None (EF_vstore chunk) (Tcons typtr (Tcons ty Tnil))
-                    (Eaddrof l typtr :: r :: nil)
-  end.
-
 (** Given a simple l-value expression [l], determine whether it
     designates a bitfield.  *)
 
@@ -200,6 +163,67 @@ Definition is_bitfield_access (l: expr) : mon bitfield :=
       | _ => error (msg "is_bitfield_access")
       end
   | _ => ret Full
+  end.
+
+(** According to the CompCert C semantics, an access to a l-value of
+    volatile-qualified type can either
+  - produce an event in the trace of observable events, or
+  - produce no event and behave as if no volatile qualifier was there.
+
+    The latter case, where the volatile qualifier is ignored, happens if
+  - the l-value is a struct or union
+  - the l-value is an access to a bit field.
+
+    The [chunk_for_volatile_type] function distinguishes between the two
+    cases.  It returns [Some chunk] if the semantics is to produce
+    an observable event of the [Event_vload chunk] or [Event_vstore chunk]
+    kind.  It returns [None] if the semantics is that of a non-volatile
+    access. *)
+
+Definition chunk_for_volatile_type (ty: type) (bf: bitfield) : option memory_chunk :=
+  if type_is_volatile ty then
+    match access_mode ty with
+    | By_value chunk =>
+        match bf with
+        | Full => Some chunk
+        | Bits _ _ _ _ => None
+        end
+    | _ => None
+    end
+  else None.
+
+(** Generate a [Sset] or [Sbuiltin] operation as appropriate
+  to dereference a l-value [l] and store its result in temporary variable [id]. *)
+
+Definition make_set (bf: bitfield) (id: ident) (l: expr) : statement :=
+  match chunk_for_volatile_type (typeof l) bf with
+  | None => Sset id l
+  | Some chunk =>
+      let typtr := Tpointer (typeof l) noattr in
+      Sbuiltin (Some id) (EF_vload chunk) (Tcons typtr Tnil) ((Eaddrof l typtr):: nil)
+  end.
+
+(** Translation of a "valof" operation.
+  If the l-value accessed is of volatile type, we go through a temporary. *)
+
+Definition transl_valof (ty: type) (l: expr) : mon (list statement * expr) :=
+  if type_is_volatile ty
+  then do t <- gensym ty;
+       do bf <- is_bitfield_access l;
+       ret (make_set bf t l :: nil, Etempvar t ty)
+  else ret (nil, l).
+
+(** Translation of an assignment. *)
+
+Definition make_assign (bf: bitfield) (l r: expr) : statement :=
+  match chunk_for_volatile_type (typeof l) bf with
+  | None =>
+      Sassign l r
+  | Some chunk =>
+      let ty := typeof l in
+      let typtr := Tpointer ty noattr in
+      Sbuiltin None (EF_vstore chunk) (Tcons typtr (Tcons ty Tnil))
+                    (Eaddrof l typtr :: r :: nil)
   end.
 
 (** Translation of the value of an assignment expression.
@@ -380,17 +404,17 @@ Fixpoint transl_expr (dst: destination) (a: Csyntax.expr) : mon (list statement 
   | Csyntax.Eassign l1 r2 ty =>
       do (sl1, a1) <- transl_expr For_val l1;
       do (sl2, a2) <- transl_expr For_val r2;
+      do bf <- is_bitfield_access a1;
       let ty1 := Csyntax.typeof l1 in
       let ty2 := Csyntax.typeof r2 in
       match dst with
       | For_val | For_set _ =>
           do t <- gensym ty1;
-          do bf <- is_bitfield_access a1;
           ret (finish dst
-                 (sl1 ++ sl2 ++ Sset t (Ecast a2 ty1) :: make_assign a1 (Etempvar t ty1) :: nil)
+                 (sl1 ++ sl2 ++ Sset t (Ecast a2 ty1) :: make_assign bf a1 (Etempvar t ty1) :: nil)
                  (make_assign_value bf (Etempvar t ty1)))
       | For_effects =>
-          ret (sl1 ++ sl2 ++ make_assign a1 a2 :: nil,
+          ret (sl1 ++ sl2 ++ make_assign bf a1 a2 :: nil,
                dummy_expr)
       end
   | Csyntax.Eassignop op l1 r2 tyres ty =>
@@ -398,32 +422,33 @@ Fixpoint transl_expr (dst: destination) (a: Csyntax.expr) : mon (list statement 
       do (sl1, a1) <- transl_expr For_val l1;
       do (sl2, a2) <- transl_expr For_val r2;
       do (sl3, a3) <- transl_valof ty1 a1;
+      do bf <- is_bitfield_access a1;
       match dst with
       | For_val | For_set _ =>
           do t <- gensym ty1;
-          do bf <- is_bitfield_access a1;
           ret (finish dst
                  (sl1 ++ sl2 ++ sl3 ++
                   Sset t (Ecast (Ebinop op a3 a2 tyres) ty1) ::
-                  make_assign a1 (Etempvar t ty1) :: nil)
+                  make_assign bf a1 (Etempvar t ty1) :: nil)
                  (make_assign_value bf (Etempvar t ty1)))
       | For_effects =>
-          ret (sl1 ++ sl2 ++ sl3 ++ make_assign a1 (Ebinop op a3 a2 tyres) :: nil,
+          ret (sl1 ++ sl2 ++ sl3 ++ make_assign bf a1 (Ebinop op a3 a2 tyres) :: nil,
                dummy_expr)
       end
   | Csyntax.Epostincr id l1 ty =>
       let ty1 := Csyntax.typeof l1 in
       do (sl1, a1) <- transl_expr For_val l1;
+      do bf <- is_bitfield_access a1;
       match dst with
       | For_val | For_set _ =>
           do t <- gensym ty1;
           ret (finish dst
-                 (sl1 ++ make_set t a1 ::
-                  make_assign a1 (transl_incrdecr id (Etempvar t ty1) ty1) :: nil)
+                 (sl1 ++ make_set bf t a1 ::
+                  make_assign bf a1 (transl_incrdecr id (Etempvar t ty1) ty1) :: nil)
                  (Etempvar t ty1))
       | For_effects =>
           do (sl2, a2) <- transl_valof ty1 a1;
-          ret (sl1 ++ sl2 ++ make_assign a1 (transl_incrdecr id a2 ty1) :: nil,
+          ret (sl1 ++ sl2 ++ make_assign bf a1 (transl_incrdecr id a2 ty1) :: nil,
                dummy_expr)
       end
   | Csyntax.Ecomma r1 r2 ty =>
